new HSalsa20 interface

code/api/Hacl.Box.ZeroPad.fst
@@ -33,7 +33,7 @@ let crypto_box_beforenm k pk sk =
   let hsalsa_n = sub tmp 32ul 16ul in
   (* Compute shared key *)
   Curve25519.crypto_scalarmult hsalsa_k sk pk;
-  Hacl.Symmetric.HSalsa20.crypto_core_hsalsa20 k hsalsa_n hsalsa_k;
+  HSalsa20.hsalsa20 k hsalsa_k hsalsa_n;
   pop_frame();
   0ul
 
@@ -88,7 +88,7 @@ let crypto_box_detached c mac m mlen n pk sk =
   Curve25519.crypto_scalarmult k sk pk;
   let h1 = ST.get() in
   cut (modifies_0 h0 h1);
-  Hacl.Symmetric.HSalsa20.crypto_core_hsalsa20 subkey hsalsa_n k;
+  HSalsa20.hsalsa20 subkey k hsalsa_n;
   let h2 = ST.get() in
   cut (modifies_0 h0 h2);
   let z = crypto_secretbox_detached c mac m mlen n subkey in
@@ -120,7 +120,7 @@ let crypto_box_open_detached m c mac mlen n pk sk =
   let hsalsa_n = sub key 64ul 16ul in
   (* Compute shared key *)
   Curve25519.crypto_scalarmult k sk pk;
-  Hacl.Symmetric.HSalsa20.crypto_core_hsalsa20 subkey hsalsa_n k;
+  HSalsa20.hsalsa20 subkey k hsalsa_n;
   let z = crypto_secretbox_open_detached m c mac mlen n subkey in
   pop_frame();
   z
