code/salsa-family/interfaces/HSalsa20.fsti
@@ -1,0 +1,26 @@
+module HSalsa20
+
+
+open FStar.Buffer
+open Spec.HSalsa20
+open Hacl.Spec.Endianness
+
+
+let h32     = Hacl.UInt32.t
+let u32     = FStar.UInt32.t
+let uint8_p = buffer Hacl.UInt8.t
+let state   = b:buffer h32{length b = 16}
+
+#reset-options "--max_fuel 0 --max_ifuel 0"
+
+let op_String_Access h (b:uint8_p{live h b}) = reveal_sbytes (as_seq h b)
+
+val hsalsa20:
+  output:uint8_p{length output = 32} ->
+  key:uint8_p{length key = 32} ->
+  nonce:uint8_p{length nonce = 16} ->
+  Stack unit
+    (requires (fun h -> live h output /\ live h nonce /\ live h key))
+    (ensures  (fun h0 _ h1 -> live h0 output /\ live h0 nonce /\ live h0 key /\
+      modifies_1 output h0 h1 /\ live h1 output
+      /\ (h1.[output] == hsalsa20 h0.[key] h0.[nonce])))
